tests/src/dynamic_size.rs
@@ -1,7 +1,6 @@
 //@ [!lean] skip
 
-
-fn alloc_slice<const N : usize>() -> Box<[u8]> {
+fn alloc_slice<const N: usize>() -> Box<[u8]> {
     Box::new([0; N])
 }
 
@@ -9,6 +8,6 @@ pub struct Wrapper<T: ?Sized> {
     data: T,
 }
 
-fn alloc_wrapper<const N : usize>() -> Box<Wrapper<[u8]>> {
-    Box::new(Wrapper{data: [0; N]})
+fn alloc_wrapper<const N: usize>() -> Box<Wrapper<[u8]>> {
+    Box::new(Wrapper { data: [0; N] })
 }
