tests/src/vec.rs
@@ -9,3 +9,7 @@ fn use_extend_from_slice<T: Clone>(v: &mut Vec<T>, s: &[T]) {
 fn use_alloc_with_capacity<T>(n: usize) -> Vec<T> {
     Vec::with_capacity(n)
 }
+
+fn from_elem<T: Clone>(x: T, n: usize) -> Vec<T> {
+    std::vec::from_elem(x, n)
+}
