backends/lean/Aeneas/Std/Array/Core.lean
@@ -1,7 +1,10 @@
 /- Arrays/Slices -/
 import Aeneas.Std.Scalar.Core
+import Aeneas.List.List
 
 namespace Aeneas.Std
+
+open Result
 
 /-!
 # Notations for `List`
@@ -11,5 +14,36 @@ instance {α : Type u} : GetElem (List α) Usize α (fun l i => i.val < l.length
 
 instance {α : Type u} : GetElem? (List α) Usize α (fun l i => i < l.length) where
   getElem? l i := getElem? l i.val
+
+/-
+# Theorems
+-/
+theorem List.mapM_clone_eq {T : Type u} {clone : T → Result T} {l : List T}
+  (h : ∀ x ∈ l, clone x = ok x) :
+  List.mapM clone l = ok l := by
+  have hind (l acc : List T) (h : ∀ x ∈ l, clone x = ok x) :
+    List.mapM.loop clone l acc = ok (List.reverse acc ++ l) := by
+    revert acc
+    induction l <;> intro acc <;> simp_all only [List.not_mem_nil, IsEmpty.forall_iff, implies_true,
+      List.append_nil, List.mem_cons, or_true, forall_const, forall_eq_or_imp] <;> unfold List.mapM.loop
+    . simp only [pure]
+    . rename_i hd tl ih
+      simp only [List.reverse_cons, List.append_assoc, List.cons_append, List.nil_append,
+        bind_tc_ok, h, ih]
+  apply hind
+  apply h
+
+def List.clone (clone : α → Result α) (l : List α) : Result ({ l' : List α // l'.length = l.length}) :=
+  match h :List.mapM clone l with
+  | ok v => ok ⟨ v, by have := List.mapM_Result_length h; scalar_tac ⟩
+  | fail e => fail e
+  | div => div
+
+@[progress]
+def List.clone_spec {clone : α → Result α} {l : List α} (h : ∀ x ∈ l, clone x = ok x) :
+  ∃ l', List.clone clone l = ok l' ∧ l'.val = l ∧ l'.val.length = l.length := by
+  simp only [List.clone]
+  have := List.mapM_clone_eq h
+  split <;> simp_all
 
 end Aeneas.Std
